fixed awalk_cost_neg

checker-isa19/ShortestPathNegCVerification.thy
@@ -25,12 +25,12 @@ type_synonym ICost = "IEdge_Id \<Rightarrow> 32 signed word"
 type_synonym IGraph = "32 word \<times> 32 word \<times> (IEdge_Id \<Rightarrow> IEdge)"
 (* for locale 3 *)
 type_synonym IPath = "IEdge_Id list"
-type_synonym ICycle = "IVertex \<times> 32 word \<times> IPath"
-type_synonym ICycle_Set = "32 word \<times> (ICycle list)"
+type_synonym ICycle = "IVertex \<times> IPath"
+type_synonym ICycle_Set = "ICycle list"
 
 type_synonym IPathPtr = "32 word ptr"
 type_synonym ICycle' = "IVertex \<times> 32 word \<times> IPathPtr"
-type_synonym ICycle_Set' = "32 word \<times> (ICycle' list)"
+type_synonym ICycle_Set' = "ICycle' list"
 
 abbreviation ivertex_cnt :: 
   "IGraph \<Rightarrow> 32 word"
@@ -61,16 +61,16 @@ abbreviation icycle_start ::
   "ICycle \<Rightarrow> 32 word"
 where
   "icycle_start C \<equiv> fst C"
-
+(*
 abbreviation icycle_length ::
   "ICycle \<Rightarrow> 32 word"
 where
   "icycle_length C \<equiv> fst (snd C)"
-
+*)
 abbreviation icycle_path ::
   "ICycle \<Rightarrow> IPath"
 where
-  "icycle_path C \<equiv> snd (snd C)"
+  "icycle_path C \<equiv> snd C"
 
 abbreviation icycle'_start ::
   "ICycle' \<Rightarrow> 32 word"
@@ -86,7 +86,7 @@ abbreviation icycle'_path ::
   "ICycle' \<Rightarrow> IPathPtr"
 where
   "icycle'_path C \<equiv> snd (snd C)"
-
+(*
 abbreviation icycles_num ::
   "ICycle_Set \<Rightarrow> 32 word"
 where
@@ -104,7 +104,7 @@ where
 abbreviation icycles' :: "ICycle_Set' \<Rightarrow> ICycle' list"
 where
   "icycles' CS \<equiv> snd CS"
-
+*)
 
 (* Implementation functions to lists *)
 
@@ -179,11 +179,12 @@ fun mk_icycle_list ::
 where 
   "mk_icycle_list CS = mk_list' (unat (icycles_num CS)) (icycles CS)"
 *)
-
+(*
 fun mk_icycle_list ::
   "ICycle_Set \<Rightarrow> ICycle list"
 where
   "mk_icycle_list CS = icycles CS"
+*)
 (*
 fun mk_icycle'_list :: 
   "ICycle_Set' \<Rightarrow> ICycle' list"
@@ -191,12 +192,22 @@ where
   "mk_icycle'_list CS = mk_list' (unat (icycles'_num CS)) (icycles' CS)"
 *)
 
+(*
 fun mk_icycle'_list ::
 "ICycle_Set' \<Rightarrow> ICycle' list"
 where
 "mk_icycle'_list CS = icycles' CS"
-
+*)
 (*Helper word lemmas*)
+
+lemma word_nat_simp[simp]:
+  assumes "(a :: 32 word) < max_word"
+  shows "unat (a + 1) = unat a + 1"
+  by(insert assms less_is_non_zero_p1 word_overflow_unat, blast)
+
+lemma word_max_limit_simp[simp]:
+  "unat (x :: 32 word) \<le> unat (max_word :: 32 word)"
+  using word_le_nat_alt by blast
 
 lemma sint_ucast: 
   "sint (ucast (x ::word32) :: sword32) = sint x"
@@ -535,23 +546,26 @@ fun abs_ICycle' ::
 where
   "abs_ICycle' h iC' = 
         (icycle'_start iC', 
-         icycle'_length iC', 
          mk_ipath'_list h iC')"
 
-abbreviation is_path
+abbreviation 
+  is_path :: "'a lifted_globals_scheme \<Rightarrow> IPath \<Rightarrow> 32 word ptr \<Rightarrow> bool"
 where
-  "is_path h iC p \<equiv> 
-        arrlist (heap_w32 h) (is_valid_w32 h) (mk_ipath_list iC) p"
+  "is_path h iP p \<equiv> 
+        arrlist (heap_w32 h) (is_valid_w32 h) iP p"
 
-definition is_cycle'
+definition 
+  is_cycle' :: "'a lifted_globals_scheme \<Rightarrow> ICycle' \<Rightarrow> Cycle_C ptr \<Rightarrow> bool"
 where
   "is_cycle' h iC' p \<equiv>
     is_valid_Cycle_C h p \<and> 
     icycle'_start iC' = start_C (heap_Cycle_C h p) \<and> 
     icycle'_length iC' = length_C (heap_Cycle_C h p) \<and>
-    icycle'_path iC' = path_C (heap_Cycle_C h p)"
+    icycle'_path iC' = path_C (heap_Cycle_C h p) \<and>
+    (\<forall>i<unat (icycle'_length iC'). 
+       is_valid_w32 h ((icycle'_path iC') +\<^sub>p int i))"
 
-
+(*
 definition 
   from_icycle'_to_icycle_list ::
   "'a lifted_globals_scheme \<Rightarrow> ICycle'\<Rightarrow> ICycle \<Rightarrow> bool"
@@ -569,7 +583,17 @@ where
     unat (icycle_length iC) = length (icycle_path iC) \<and>
     icycle_length iC = length_C (heap_Cycle_C h p) \<and>
     is_path h iC (path_C (heap_Cycle_C h p))"
+*)
 
+definition 
+  is_cycle :: "'a lifted_globals_scheme \<Rightarrow> ICycle \<Rightarrow> Cycle_C ptr \<Rightarrow> bool"
+where
+  "is_cycle h iC p \<equiv>
+    is_valid_Cycle_C h p \<and> 
+    icycle_start iC = start_C (heap_Cycle_C h p) \<and> 
+    length (icycle_path iC) = unat (length_C (heap_Cycle_C h p)) \<and>
+    is_path h (icycle_path iC) (path_C (heap_Cycle_C h p))"
+(*
 definition final_is_cycle
 where
   "final_is_cycle h iC' p \<equiv>
@@ -577,21 +601,24 @@ where
     icycle'_start iC' = start_C (heap_Cycle_C h p) \<and>
     icycle'_length iC' = length_C (heap_Cycle_C h p) \<and>
     is_path h (abs_ICycle' h iC') (path_C (heap_Cycle_C h p))"
+*)
 
-definition abs_ICycles' :: 
-  "'a lifted_globals_scheme \<Rightarrow> ICycle_Set' \<Rightarrow> ICycle_Set"
+definition 
+  abs_ICycles' :: "'a lifted_globals_scheme \<Rightarrow> ICycle_Set' \<Rightarrow> ICycle_Set"
 where
-  "abs_ICycles' h CS' \<equiv> 
-    (icycles'_num CS', 
-     map (abs_ICycle' h) (icycles' CS'))"
+  "abs_ICycles' h CS' \<equiv> map (abs_ICycle' h)  CS'"
 
-definition are_cycles'
+definition 
+  are_cycles' :: 
+  "'a lifted_globals_scheme \<Rightarrow> ICycle_Set' \<Rightarrow> Cycle_set_C ptr \<Rightarrow> bool"
 where
   "are_cycles' h iCS' p \<equiv>
     is_valid_Cycle_set_C h p \<and>
-    icycles'_num iCS' = no_cycles_C (heap_Cycle_set_C h p) \<and> 
+    length iCS' = unat (no_cycles_C (heap_Cycle_set_C h p)) \<and> 
     arrlist (heap_Cycle_C h) (is_valid_Cycle_C h)
-       (map to_cycle (icycles' iCS'))  (cyc_obj_C (heap_Cycle_set_C h p))"
+       (map to_cycle iCS') (cyc_obj_C (heap_Cycle_set_C h p)) \<and>
+    (\<forall>i<length iCS'. 
+       is_valid_w32 h (icycle'_path (iCS'! i)))"
 
 (*
 definition are_cycles
@@ -684,12 +711,12 @@ where
   "abs_IPath \<equiv> id"
 *)
 
-
+(*
 definition abs_ICycle :: 
   "ICycle_Set \<Rightarrow> (32 word \<times> (32 word awalk)) set"
 where
   "abs_ICycle CS \<equiv> set (map (\<lambda> C. (icycle_start C, icycle_path C)) (icycles CS))"
-
+*)
 lemma None_abs_pedgeI[simp]:
   "(abs_IPedge p v = None) = msb (p v)"
   using abs_IPedge_def by auto
@@ -837,61 +864,6 @@ lemma arrlist_next_item:
   shows "arrlist h v xs (p +\<^sub>p 1)"
   using assms by simp
 
-lemma ipathptr_ipath_simp:
-  "\<lbrakk> hp = heap_w32 h; v = is_valid_w32 h; (x # xs) = mk_ipath h p l; 
-     v p \<rbrakk> \<Longrightarrow> arrlist hp v xs p"
-(*
-  apply clarsimp
-  apply (induct hp v xs p arbitrary: p l rule: arrlist.induct)
-   apply simp
-  apply clarsimp
-  apply safe
-   apply (metis array_addrs.simps(2) length_Cons list.inject array_addrs_length)
-  apply (erule_tac x="pa" in meta_allE)
-  apply (erule_tac x="l" in meta_allE)
-  apply clarsimp
-*)
-  (* HERE *)
-
-
-  sorry
-(*
-lemma ipathptr_ipath_simp2:
-  "\<lbrakk> heap_w32 h p; is_valid_w32 h p \<rbrakk> \<Longrightarrow> arrlist (heap_w32 h) (is_valid_w32 h) (mk_ipath h p l) p"
-  apply (induct "(mk_ipath h p l)" arbitrary: p)
-   apply clarsimp
-  
-  apply (case_tac l)
-   apply (simp)
-  apply (simp add:array_addrs.simps(2))+
-  apply (erule_tac x="p" in meta_allE)
-   apply (simp add:array_addrs.simps(2))
-  apply(metis (no_types) array_addrs.simps(2) arrlist.simps(2) list.simps(9) ipathptr_ipath_simp mk_ipath.simps)
-  sorry
-
-*)
-
-
-
-
-
-lemma ipathptr_ipath_simp:
-  "\<lbrakk> hp = heap_w32 h; v = is_valid_w32 h; (x # xs) = mk_ipath h p l; 
-     v p \<rbrakk> \<Longrightarrow> arrlist hp v xs p"
-(*
-  apply clarsimp
-  apply (induct hp v xs p arbitrary: p l rule: arrlist.induct)
-   apply simp
-  apply clarsimp
-  apply safe
-   apply (metis array_addrs.simps(2) length_Cons list.inject array_addrs_length)
-  apply (erule_tac x="pa" in meta_allE)
-  apply (erule_tac x="l" in meta_allE)
-  apply clarsimp
-*)
-  oops
-
-
 lemma arrlist_array_addrs:
   "\<lbrakk>\<forall>i<n. v (p +\<^sub>p int i); xs= map h (array_addrs p n)\<rbrakk> \<Longrightarrow> arrlist h v xs p"
   apply (induct n arbitrary: p xs) 
@@ -901,29 +873,17 @@ lemma arrlist_array_addrs:
   apply (frule_tac x=0 in spec, simp)
   by force
 
-(*
-lemma temp:
-  "arrlist (heap_w32 h) (is_valid_w32 h) 
-    (map (heap_w32 h)   
-      (array_addrs (icycle'_path iC') 
-     (unat (icycle'_length iC'))))
-     (icycle'_path iC')"
-  sorry
-*)
-lemma is_path_absICycle': (*ipathptr_ipath_simp:*)
+lemma is_path_absICycle':
   "\<forall>i<unat (icycle'_length iC'). 
        is_valid_w32 h ((icycle'_path iC') +\<^sub>p int i) \<Longrightarrow>
-       is_path h (abs_ICycle' h iC') (icycle'_path iC')"
+       is_path h (icycle_path (abs_ICycle' h iC')) (icycle'_path iC')"
   by (simp add: arrlist_array_addrs)
 
-
-lemma icycle'_to_icycle_simp:
-  "\<forall>i<unat (icycle'_length iC'). 
-       is_valid_w32 h ((icycle'_path iC') +\<^sub>p int i) \<Longrightarrow>
-   from_icycle'_to_icycle_list h iC' (abs_ICycle' h iC')"
-  unfolding from_icycle'_to_icycle_list_def 
-  using is_path_absICycle'
-  by force
+lemma is_icycle'_is_icycle:
+  "\<lbrakk>is_cycle' h iC' p\<rbrakk> \<Longrightarrow> is_cycle h (abs_ICycle' h iC') p"
+  unfolding is_cycle'_def is_cycle_def 
+  using is_path_absICycle' 
+  by (clarsimp simp: array_addrs_length) 
 
 lemma word_less_arith_simp[simp]:
   "\<lbrakk> x \<noteq> 0; (x :: 32 word) < l \<rbrakk> \<Longrightarrow> (x - 1) < l"
@@ -981,7 +941,7 @@ lemma awalk_spc':
                    yy \<le> icycle_length iY \<and> 
                    wf_digraph (abs_IGraph iG) \<and>
                    is_graph s iG g \<and>
-                   is_cycle s iY y"])
+                   is_cycle s iY y"]) sorry
   apply (simp add: skipE_def)
   apply wp 
         apply (subst if_bool_eq_conj)+ 
@@ -1007,125 +967,113 @@ lemma awalk_spc':
   sorry
 
 definition awalk_cost_neg_inv ::
-  "ICost \<Rightarrow> ICycle \<Rightarrow> 32 word \<Rightarrow> int"
+  "ICost \<Rightarrow> ICycle \<Rightarrow> nat \<Rightarrow> int"
 where
   "awalk_cost_neg_inv iC iY ee \<equiv> 
-      sum_list (map (sint \<circ> iC) (take (unat ee) (icycle_path iY)))"
+      sum_list (map (sint \<circ> iC) (take ee (icycle_path iY)))"
 
 lemma sum_list_step:
-  assumes "(i + 1) \<le> length xs" 
+  assumes "i < length xs" 
   assumes "xs \<noteq> []"
   shows "sum_list (take (i + 1) xs) = sum_list (take i xs) + xs ! i"
 proof -
   have "\<forall>n. n + 1 = Suc n"
     by simp
   then show ?thesis
-    by (metis (no_types) add.right_neutral assms(1) le_less_trans lessI not_le sum_list.Cons sum_list.Nil sum_list_append take_Suc_conv_app_nth)
+    by (metis (no_types) add.right_neutral assms(1) sum_list.Cons sum_list.Nil sum_list_append take_Suc_conv_app_nth)
 qed
 
 lemma sum_list_step_sint:
-  assumes "(i + 1) \<le> length xs" 
+  assumes "i < length xs" 
   assumes "xs \<noteq> []"
   shows "sum_list (map sint (take (i + 1) xs)) = sum_list (map sint (take i xs)) + sint (xs ! i)"
 proof -
   have "sum_list (take i (map sint xs)) + sint (xs ! i) = sum_list (take (i + 1) (map sint xs))"
-    by (metis (no_types) add.commute assms(1) discrete gen_length_code(1) gen_length_def length_map not_add_less1 nth_map sum_list_step)
+    by (metis (no_types) add.commute assms(1) gen_length_code(1) gen_length_def length_map not_add_less1 nth_map sum_list_step)
   then show ?thesis
     by (simp add: take_map)
 qed
 
 lemma awalk_cost_neg_inv_step:
-  assumes i_less_max: "i < (max_word::32 word)"
-    and "unat (fst (snd iY)) = length (snd (snd iY))"
-    and "(i + 1) \<le> icycle_length iY"
-    and "icycle_path iY \<noteq> []"
+  assumes "is_cycle s iY y"
+    and   "i  < (length (icycle_path iY))"
+    and   "icycle_path iY \<noteq> []"
   shows "awalk_cost_neg_inv iC iY (i + 1) = awalk_cost_neg_inv iC iY i +
-  sint (map iC (icycle_path iY) ! unat i)"
-  apply (insert assms)
-  apply (unfold awalk_cost_neg_inv_def)
-  apply (subgoal_tac "sum_list (map sint (take (unat (i + 1)) (map iC (snd (snd iY))))) =
-        sum_list (map sint (take (unat i) (map iC (snd (snd iY))))) + sint (map iC (icycle_path iY) ! unat i)")
+  sint (map iC (icycle_path iY) !  i)"
+  unfolding awalk_cost_neg_inv_def is_cycle_def
+  using  assms
+  apply (subgoal_tac "sum_list (map sint (take (i + 1) 
+          (map iC (icycle_path iY)))) =
+        sum_list (map sint (take i (map iC (icycle_path iY)))) + 
+         sint (map iC (icycle_path iY) ! i)")
   apply (simp add: take_map)
-  apply (subgoal_tac "\<forall>w. (w::32 word) = 0 \<or> \<not> unat w < 1 + unat (0::32 word)")
-   apply (subgoal_tac "1 + unat (0::32 word) = 1 \<or> (0::32 word) = 1")
-    apply (subgoal_tac "\<not> fst (snd iY) < i + 1")
-     apply (metis (no_types) Nil_is_map_conv add.commute length_map less_is_non_zero_p1 not_le unat_simp 
-            sum_list_step_sint unat_1 word_less_nat_alt word_not_simps(1))
-    apply simp
-   apply simp
-  apply (metis add.commute discrete less_linear not_le word_less_nat_alt word_not_simps(1))
+  apply (metis (no_types, lifting) 
+        Nil_is_map_conv add.commute length_map sum_list_step_sint)
   done
 
 corollary awalk_cost_neg_inv_step2:
-  assumes i_less_max: "i < (max_word::32 word)"
-    and "unat (fst (snd iY)) = length (snd (snd iY))"
-    and "(i + 1) \<le> icycle_length iY"
+  assumes "is_cycle s iY y"
+    and "i < length (icycle_path iY)"
     and "icycle_path iY \<noteq> []"
   shows "awalk_cost_neg_inv iC iY (i + 1) = awalk_cost_neg_inv iC iY i +
-  sint (iC (icycle_path iY ! unat i))"
-  apply (insert assms)
-  apply (unfold awalk_cost_neg_inv_def)
-  apply (subgoal_tac "sint (iC (icycle_path iY ! unat i)) = sint (map iC (icycle_path iY) ! unat i)")
-   apply clarsimp 
-   apply (metis awalk_cost_neg_inv_def awalk_cost_neg_inv_step)
-  apply (metis (no_types, hide_lams) max_word_not_less nth_map word_Suc_le word_less_nat_alt)
-  done
+  sint (iC (icycle_path iY ! i))"
+  unfolding awalk_cost_neg_inv_def
+  using assms awalk_cost_neg_inv_def awalk_cost_neg_inv_step
+  by (metis (no_types, hide_lams) One_nat_def add_Suc_right nth_map
+              gen_length_code(1) gen_length_def list.size(3))
 
 lemma awalk_cost_neg_spc':
-  "ovalid (\<lambda> s. (\<forall>i < icycle_length iY. icycle_path iY ! unat i < iedge_cnt iG) \<and>
-   wf_digraph (abs_IGraph iG) \<and>
+  "ovalid (\<lambda> s. (\<forall>i < length (icycle_path iY). 
+   icycle_path iY ! i < iedge_cnt iG) \<and>
    is_graph s iG g \<and>
    is_cost s iG iC c \<and>
-   is_cycle s iY y) (awalk_cost_neg' c y) (\<lambda>r s. r = awalk_cost_neg_inv iC iY (icycle_length iY))"
+   is_cycle s iY y) (awalk_cost_neg' c y) (\<lambda>r s. r = 
+   awalk_cost_neg_inv iC iY (length (icycle_path iY)))"
   apply (unfold awalk_cost_neg_inv_def awalk_cost_neg'_def)[1]
-  apply (subst owhile_add_inv[where M="\<lambda> (ee, total) s. unat (icycle_length iY - ee)" and
+  apply (subst owhile_add_inv [where 
+         M="\<lambda> (ee, total) s. (length (icycle_path iY) - unat ee)" and
          I="\<lambda> (ee, total) s. 
-              (\<forall>i < icycle_length iY. icycle_path iY ! unat i < iedge_cnt iG) \<and>
-              ee \<le> icycle_length iY \<and>
-              wf_digraph (abs_IGraph iG) \<and>
+              length (icycle_path iY) \<le> unat (max_word::32 word) \<and>
+              (\<forall>i < length (icycle_path iY). icycle_path iY ! i < iedge_cnt iG) \<and>
               is_graph s iG g \<and>
               is_cost s iG iC c \<and>
               is_cycle s iY y \<and>
-              total = awalk_cost_neg_inv iC iY ee"])
+              total = awalk_cost_neg_inv iC iY (unat ee)"])
   apply wpsimp
-    apply (subgoal_tac "a < (max_word::32 word)")
-     apply (drule awalk_cost_neg_inv_step2[where iC=iC and iY="iY"])
-        apply (unfold awalk_cost_neg_inv_def)[1] 
-        apply blast
-       apply (simp add: inc_le is_cycle_def)
-      apply (unfold is_cycle_def, clarsimp)[1]
-      apply (simp add: word_less_nat_alt)
-     apply (rule conjI)
-      apply (simp add: inc_le is_cycle_def)
-     apply (unfold is_cycle_def is_cost_def)[1]
-     apply clarsimp 
-     apply (subst arrlist_heap[where iL=iC]) 
-       apply blast
-      apply clarsimp
-     apply (simp add: arrlist_cycle_path_heap)
-     apply (simp add: arrlist_cycle_path_heap uint_nat word_less_nat_alt)
-    apply (metis max_word_not_less not_le word_minus_one_le)
+    apply (frule_tac i="unat a" in 
+      awalk_cost_neg_inv_step2[where iC=iC and iY="iY"]) 
+      apply (fastforce intro: unat_mono simp: is_cycle_def)
+     apply (metis add.right_neutral list.size(3) not_add_less2 is_cycle_def word_less_nat_alt)
+    apply (subgoal_tac "a < (max_word :: 32 word)")
+     apply (subst (asm) word_nat_simp[symmetric], fast)
+     apply (clarsimp simp add: awalk_cost_neg_inv_def is_cycle_def is_cost_def)
+     apply (subst (asm) arrlist_cycle_path_heap, blast, fastforce simp add: word_less_nat_alt)
+     apply (subst (asm) arrlist_heap[where iL=iC], fast, metis arrlist_cycle_path_heap word_less_nat_alt)
+     apply (simp add: uint_nat)
+     apply (subst arrlist_cycle_path_heap, blast, fastforce simp add: word_less_nat_alt)
+     apply (subst arrlist_heap[where iL=iC], fast, metis arrlist_cycle_path_heap word_less_nat_alt)
+     apply clarsimp
+    apply (insert less_linear max_word_not_less, blast)
    apply wpsimp
-   apply (simp add: is_cycle_def awalk_cost_neg_inv_def)
+   apply (clarsimp simp add: awalk_cost_neg_inv_def is_cycle_def)
+   apply (insert word_le_nat_alt word_le_not_less, fastforce)
   apply wpsimp
-  apply (unfold awalk_cost_neg_inv_def)
-  apply clarsimp
+  apply (clarsimp simp add: is_cycle_def awalk_cost_neg_inv_def)
   done
 
 lemma int_real_add_simp: "foldr (+) (map (real_of_int \<circ> sint) xs) 0 = 
                           real_of_int (foldr (+) (map sint xs) 0)"
   by (induct xs) simp+
 
-lemma acc_list_simp: "real_of_int (awalk_cost_neg_inv iC iY (icycle_length iY)) = 
-       sum_list (map (real_of_int \<circ> sint \<circ> iC) (take (unat (fst (snd iY))) (icycle_path iY)))"
+lemma acc_list_simp: "real_of_int (awalk_cost_neg_inv iC iY (length (icycle_path iY))) = 
+       sum_list (map (real_of_int \<circ> sint \<circ> iC) (take (length (icycle_path iY)) (icycle_path iY)))"
   unfolding awalk_cost_neg_inv_def
   using int_real_add_simp 
   by (metis (no_types, hide_lams) map_map sum_list.eq_foldr)
 
 lemma awalk_cost_eq_math:
   assumes "wf_digraph (abs_IGraph iG)"
-  assumes "unat (icycle_length iY) = length (icycle_path iY)"
-  shows "real_of_int (awalk_cost_neg_inv iC iY (icycle_length iY)) = wf_digraph.awalk_cost (abs_ICost iC) (icycle_path iY)"
+  shows "real_of_int (awalk_cost_neg_inv iC iY (length (icycle_path iY))) = wf_digraph.awalk_cost (abs_ICost iC) (icycle_path iY)"
   apply (insert assms)
   apply (simp add: acc_list_simp)
   apply (unfold awalk_inv_def awalk_cost_neg_inv_def wf_digraph.awalk_cost_def abs_ICost_def)
